only pose purified hyp if it doesn't follow by xlia zchecker,
and before presenting the goal to the user, when deciding
which purified hyps to keep, delete them upwards starting from
derivability_test_marker rather than downwards until the marker,
because hyps further up tend to be simpler.
Fixes two kinds of issues observed in swap_subarray.v:
- superfluous hypotheses: eg `__pure_H1: \[i] = \[i]`
- overly complicated hypotheses: eg `a1 - b - c = a2 - b - c` was
  kept, because `a1 = a2` (further up) had been deleted. Now,
  `a1 = a2` is kept, and the longer one is deleted because it follows.

LiveVerif/src/LiveVerifExamples/ring_buffer.v
@@ -22,8 +22,22 @@ typedef struct __attribute__ ((__packed__)) {
 Definition ring_buffer(cap: Z)(vs: list word)(addr: word): mem -> Prop :=
   ex1 (fun b: raw_ring_buffer =>
     sep (raw_ring_buffer_t b addr)
-        (emp (capacity b = cap /\ n_elems b = len vs /\
-             (data b ++ data b)[dequeue_pos b : dequeue_pos b + n_elems b] = vs))).
+        (emp (capacity b = cap /\
+              0 <= dequeue_pos b < cap /\
+              0 <= n_elems b <= cap /\
+              len (data b) = cap /\
+              (data b ++ data b)[dequeue_pos b : dequeue_pos b + n_elems b] = vs))).
+
+Lemma purify_ring_buffer: forall cap vs addr,
+    purify (ring_buffer cap vs addr) (len vs <= cap).
+Proof.
+  unfold purify, ring_buffer, ex1. intros. fwd.
+  repeat step_silent.
+  subst.
+  bottom_up_simpl_in_goal.
+  lia.
+Qed.
+Hint Resolve purify_ring_buffer : purify.
 
 Hint Unfold ring_buffer : live_always_unfold.
 
@@ -41,11 +55,8 @@ Derive ring_buf_enq SuchThat (fun_correct! ring_buf_enq) As ring_buf_enq_ok.    
 {                                                                          /**. .**/
   uintptr_t i = (load32(b_addr+4) + load32(b_addr+8)) % load32(b_addr);    /**.
 
-  unfold raw_ring_buffer_t in *|-.
-
-  (* interp_sepapp_tree semi-reification to expose one field *)
-
-  (* TODO support &p->field notation, which would allow writing
+  (* TODO support &p->field notation, which would allow writing this:
+     (but probably need a cast of uintptr to record type first?
   uintptr_t i = (load32(&b_addr->dequeue_pos) + load32(&b_addr->n_elems))
                 % load32(&b_addr->capacity);
 
