bedrock2/src/bedrock2/PurifyHeapletwise.v
@@ -1,28 +1,84 @@
 Require Import Ltac2.Ltac2.
 Require Import Coq.micromega.Lia.
+Require Import coqutil.Map.Interface.
+Require Import coqutil.Word.Interface.
 Require Import coqutil.Tactics.fold_hyps coqutil.Tactics.foreach_hyp.
 Require Import bedrock2.PurifySep.
 Require Import bedrock2.HeapletwiseHyps.
 Require Import coqutil.Tactics.ident_ops.
+Require Import bedrock2.bottom_up_simpl_ltac1.
 Require Import bedrock2.unzify.
 
-Ltac purify_heapletwise_pred_cont k H pred m :=
-  let pf := constr:(ltac:(eauto with purify) : purify pred _) in
-  lazymatch type of pf with
-  | purify pred True => idtac
-  | purify pred ?P =>
-      let HP := fresh "__pure_" H in pose proof (pf m H) as HP; k HP P
+Ltac is_var_b x :=
+  match constr:(Set) with
+  | _ => let __ := match constr:(Set) with
+                   | _ => is_var x
+                   end in
+         constr:(true)
+  | _ => constr:(false)
   end.
 
-Ltac purify_heapletwise_hyp_of_type_cont k H t :=
-  match t with
-  | ?R ?m => purify_heapletwise_pred_cont k H R m
-  | with_mem ?m ?R => purify_heapletwise_pred_cont k H R m
-  | _ => idtac
+(* TODO replace by simple tactic failure? *)
+Inductive nothing_to_purify: Prop := .
+
+(* returns the name of the new purified hyp or nothing_to_purify *)
+Ltac purified_hyp_name_of_pred h pred m :=
+  lazymatch is_var_b pred with
+  | true => constr:(nothing_to_purify)
+  | false =>
+      let g := open_constr:(purify pred _) in
+      let pf := match constr:(Set) with
+                | _ => constr:(ltac:(eauto with purify) : g)
+                | _ => fail 1000 g "cannot be solved by eauto with purify"
+                end in
+      lazymatch type of pf with
+      | purify pred True => constr:(nothing_to_purify)
+      | purify pred ?p =>
+          let hp := fresh "__pure_" h in
+          let __ := match constr:(Set) with
+                    | _ => pose proof (pf m h) as hp
+                    end in
+          hp
+      end
   end.
 
-Ltac purify_heapletwise_hyps :=
-  foreach_hyp (purify_heapletwise_hyp_of_type_cont ltac:(fun h tp => idtac)).
+(* returns the name of the new purified hyp or nothing_to_purify *)
+Ltac purified_hyp_name h t :=
+  lazymatch t with
+  | with_mem ?m ?pred => purified_hyp_name_of_pred h pred m
+  | ?pred ?m => lazymatch type of m with
+                | @map.rep (@word.rep _ _) Byte.byte _ => purified_hyp_name_of_pred h pred m
+                | _ => constr:(nothing_to_purify)
+                end
+  | _ => constr:(nothing_to_purify)
+  end.
+
+Ltac puri_simpli_zify_hyp fail_if_too_trivial h t :=
+  try ((* try block starts here because everthing starting from here needs
+          to be reverted if the resulting hyp is too trivial *)
+      let hp := purified_hyp_name h t in
+      lazymatch hp with
+      | nothing_to_purify => idtac
+      | _ => let tp := type of hp in
+             bottom_up_simpl_in_hyp_of_type hp tp;
+             let tp := type of hp in
+             let wok := get_word_ok_or_dummy in
+             let zo := zify_hyp_option wok hp tp in
+             assert_succeeds
+               (idtac;
+                lazymatch zo with
+                | @None ?tz => clear hp; fail_if_too_trivial tz
+                | @Some ?tz ?hz => clear hp hz; fail_if_too_trivial tz
+                end);
+             apply_range_bounding_lemma_in_eqs
+      end).
+
+(* possible arguments for fail_if_too_trivial above: *)
+Ltac accept_always t := idtac.
+Ltac accept_unless_follows_by_xlia t := assert_fails (idtac; assert t by xlia zchecker).
+
+Ltac puri_simpli_zify_hyps fail_if_too_trivial :=
+  foreach_hyp (puri_simpli_zify_hyp fail_if_too_trivial).
 
 Inductive derivability_test_marker: Prop := mk_derivability_test_marker.
 
@@ -33,20 +89,12 @@ Ltac clear_pure_hyp_if_derivable h tp :=
 
 Ltac clear_upto_marker marker :=
   lazymatch goal with
-  | H: marker |- _ =>
-      repeat lazymatch goal with
-        | A: ?T |- _ => lazymatch T with
-                        | marker => fail (* done *)
-                        | _ => clear A
-                        end
-        end;
-      clear H
-  | |- _ => fail "marker not found found"
+  | m: marker |- _ => foreach_hyp_upto_marker marker (fun h tp => clear h); clear m
+  | |- _ => fail "marker not found"
   end.
 
 Ltac unpurify :=
   pose proof mk_derivability_test_marker;
-  purify_heapletwise_hyps;
-  zify_hyps_upto_marker derivability_test_marker;
-  foreach_hyp_downto_marker derivability_test_marker clear_pure_hyp_if_derivable;
+  puri_simpli_zify_hyps accept_always;
+  foreach_hyp_from_marker_upwards derivability_test_marker clear_pure_hyp_if_derivable;
   clear_upto_marker derivability_test_marker.
